## 1.3 Radicals and Rational Exponents
#### Evaluating Square Roots
- When the square root of a number is squared, the result is the original number, such as $4^2 = 16$ so $\sqrt{16} = 4$. The square root function is the inverse of squaring a number
- Generally, if $a$ is a positive real number, then $\sqrt{a}$ is a number that, when multiplied by itself, gives $a$. The square root could be positive/negative, because multiplying two negative numbers gives a positive
- The **principal square root** is a non-negative number that when multiplied by itself equals $a$, the principal square root of $a$ is written as $\sqrt{a}$. The symbol $\sqrt{}$ is called a **radical**, the term under the symbol is the **radicand** and the entire expression is a **radical expression**
- Examples

---
In-Class notes
- In a square root, the symbol $\sqrt{}$ is the `radical`, the number under the radical is the `radicand`, and the entire expression is the `radical expression`
- If there is no number written, then there is an "invisible" two in the radical, ex. $\sqrt[2]{25}$
- In the example $\sqrt[n]{a^m}$
    - $n$ = index
    - $m$ = exponent
    - $a$ = base
    - $a^m$ = radicand
- $\sqrt{100} = 10$
- $\sqrt{\sqrt{16}} = \sqrt{4} = 2$
- $\sqrt{25 + 144} = \sqrt{169} = 13$
- $\sqrt{}$
- If a > 0 and b > 0, then $\sqrt{ab} = \sqrt{a} \cdot \sqrt{b}$
    - Similarly, $\sqrt[5]{a} \cdot \sqrt[5]{b} = \sqrt[5]{ab}$
- $\frac{\sqrt{234x^{11}y}}{\sqrt{26x7y}} = \sqrt{\frac{234x^{11}y}{26x^7y}} = \sqrt{\frac{117x^4}{13}} = \sqrt{9x^4} = 3x^2$
- $\sqrt{2} \cdot \sqrt{8} = \sqrt{2 \cdot 8} = \sqrt{16} = 4$
- $3\sqrt{17} + 2\sqrt{17} = 5\sqrt{17}$
    - Similar radicals can be combined (think of it as the same as $3x + 2x = 5x$)
- $\sqrt{5} + 6\sqrt{20}$
- $5\sqrt{2} + 3\sqrt{18} = 5\sqrt{2} + 3\sqrt{9 \cdot 2} = 5\sqrt{2} + 9\sqrt{2} = 14\sqrt{2}$
- $20\sqrt{72a^3b^4c} - 14\sqrt{8a^3b^4c} = 20\sqrt{36 \cdot 2 a^2 \cdot a^1 \cdot b^2 \cdot b^2 \cdot c} - 14\sqrt{4 \cdot 2 \cdot a^2 \cdot a \cdot b^2 \cdot b^2 \cdot c}$
    - $= 20 \cdot 6ab^2\sqrt{2ac} - 14 \cdot 2ab^2\sqrt{2ac} = 120ab^2\sqrt{2ac} - 28ab^2\sqrt{2ac} = 92ab^2\sqrt{2ac}$
- $\sqrt{a^4} = a^{\frac{4}{2}} = a^2$
- $\sqrt[3]{1000} = 10$
- This is an example of "not good technique" for simplifying square root expressions, very manual technique
    - $\sqrt{72a^7b^{11}c^5} = \sqrt{36 \cdot 2 \cdot a^2\cdot a^2\cdot a^2 \cdot a^1 \cdot b^2\cdot b^2\cdot b^2\cdot b^2\cdot b^2 \cdot b^1 \cdot c^2\cdot c^2 \cdot c^1} = 6aaabbbbbcc\sqrt{2abc} = 6a^3b^5c^2\sqrt{2abc}$
- This is an example of "good technique"
    1. Prime factorization of any numbers under the radicand
    2. Divide the exponents within the radical by the index of the radical
    3. Combine the results of refactoring
    - $\sqrt{72a^7b^{11}c^5} = \sqrt{2^3 \cdot 3^2a^7b^{11}c^5}$
        - Take the number under th radical and do prime factorization
            - ex. $72 = 2^3 \cdot 3^2$
        - Check the exponents of each prime factor
        - Divide the exponents within the radical by the index of the radical
            - $\sqrt{2^3} = 2\sqrt{2}$
            - $\sqrt{3^2} = 3$
            - $\sqrt{a^7} = a^3\sqrt{a}$
            - $\sqrt{b^{11}} = b^5\sqrt{b}$
            - $\sqrt{c^5} = c^2\sqrt{c}$
        - Combine the results of your refactoring
            - $6a^3b^5c^2\sqrt{2abc}$
        - Additional examples
            - $\sqrt[3]{a^5} = a\sqrt[3]{a^2}$
            - $\sqrt[5]{4a^4b^5c^6e^7d^8w^{13}p^{26}}$
                - Prime factorization
                    - $\sqrt[5]{4} = 2 \cdot 2 = \sqrt[5]{2^2}$
                - Divide exponents by the index
                    - $\sqrt[5]{a^4}$
                    - $\sqrt[5]{b^5} = b$
                    - $\sqrt[5]{c^6} = c\sqrt[5]{c}$
                    - $\sqrt[5]{e^7} = e\sqrt[5]{e^2}$
                    - $\sqrt[5]{d^8} = d\sqrt[5]{d^3}$
                    - $\sqrt[5]{w^{13}} = w^2\sqrt[5]{w^3}$
                    - $\sqrt[5]{p^{26}} = p^5\sqrt[5]{p}$
                - Combine
                    - $bcedw^2p^5\sqrt[5]{2^2ce^2d^3w^3p}$
            - $\sqrt[3]{432a^7b^2c^{11}de^{15}} = \sqrt[3]{2^4 \cdot 3^3 \cdot a^7b^2c^{11}de^{15}}$
                - Prime factorization
                    - $432 / 2 = 216$
                        - $216 / 2 = 108$
                            - $108 / 2 = 54$
                                - $54 / 2 = 27$
                                    - $27 / 3 = 9$
                                        - $9 / 3 = 3$
                    - result = $2^4 \cdot 3^3$
                - Divide exponents by the index
                    - $\sqrt[3]{2^4} = 2\sqrt[3]{2}$
                    - $\sqrt[3]{3^3} = 3$
                    - $\sqrt[3]{a^7} = a^2\sqrt[3]{a}$
                    - $\sqrt[3]{b^2} = \sqrt[3]{b^2}$
                    - $\sqrt[3]{c^{11}} = c^3\sqrt[3]{c^2}$
                    - $\sqrt[3]{d} = \sqrt[3]{d}$
                    - $\sqrt[3]{e^{15}} = e^5$
                - Combine
                    - $6a^2c^3e^5\sqrt[3]{2ab^2c^2d}$
- Can think of the square root as the opposite of squaring a number
    - $\sqrt{4} = 2$
    - You can however, have $-\sqrt{25} = -5$
- **PRINCIPAL SQUARE ROOT**
    - The principal square root of $a$ is the non-negative number that, when multiplied by itself, equals $a$
    - When we say $\sqrt{4}$, it is a number, and an expression, and it is only positive
        - This is different from when we say $x^2 = 4$, this is an equation and may have multiple answers
            - Ex. $x^2 = 4 = \pm2$
- **Under any square root (or any even root), the radicand must be positive**
    - You cannot say $\sqrt{-25}$, this is called "not real"
- **IMPORTANT RULE**
    - When dealing with even roots, you need to make sure that the radicand is positive, this is because the radicand could be positive or negative, so we agree that it is positive
    - $\sqrt{a^2} = |a|$
        - Absolute value indicates "distance" from zero
    - $\sqrt{(-2)^2} = |-2| = 2$
    - $\sqrt[2]{(-6)^2} = |-6| = 6$
    - $\sqrt[2]{a^{14}} = |a^7|$
    - When dealing with odd roots, you do not have the possibility of having two options
    - $\sqrt[3]{a^3}$
- Under even root, in order to continue, you must have positive radicands
### Examples
- For examples in the textbook, assume all variables are positive
- $(\frac{\sqrt{250x^2}}{\sqrt{100b^3}})(\frac{7\sqrt{b}}{\sqrt{125x}}) = \sqrt{\frac{250x^2}{100b^3}} \cdot \frac{7}{1} \cdot \sqrt{\frac{b}{125x}} = \sqrt{\frac{5x^2}{2b^3}} \cdot \frac{7}{1} \cdot \sqrt{\frac{b}{125x}} = 7 \cdot \sqrt{\frac{5 \cdot x^2}{2 \cdot b^3} \cdot \frac{6}{125x}} = 7 \cdot \sqrt{\frac{x}{2 \cdot b^2 \cdot 25}} = 7 \cdot \frac{\sqrt{x}}{5b\sqrt{2}} = \frac{7\sqrt{x}}{5b\sqrt{2}} = \frac{7\sqrt{2x}}{10b}$
    - Remember to rationalize denominator before you are done
- $\frac{15\sqrt[4]{125}}{\sqrt[4]{5}} = 15 \cdot \sqrt[4]{\frac{125}{5}} = 15 \cdot \sqrt[4]{25} = 15 \cdot \sqrt[4]{5^2} = 15\sqrt{5}$
- $3\sqrt[3]{-432} +\sqrt[3]{16} = 3\sqrt[3]{-2^4 \cdot 3^3}+\sqrt[3]{2^4} = -3 \cdot 2 \cdot 3 \cdot \sqrt[3]{2} + 2 \cdot \sqrt[3]{2} = -16\sqrt[3]{2}$
    - If you have a negative number under an odd index, the negative jumps out
    - 432 / 2
        - 216 / 2
            - 108 / 2
                - 54 / 2
                    - 27 / 3
                        - 9 / 3
                            - 3
- $\sqrt{400x^4} = \sqrt{2^45^2x^4} = 2^2 \cdot 5 \cdot x^2 = 20x^2$
    - 400 / 2
        - 200 / 2
            - 100 / 2
                - 50 / 2
                    - 25 / 5
                        - 5
- $\sqrt{4y^2} = 2|y|$
- $\sqrt{49p} = 7\sqrt{p}$
- $(144p^2q^6)^{\frac{1}{2}} = \sqrt{144p^2q^6} = 12pq^3$ (if no assumption that all variables are positive then $12|p|q^3$)
- $m^{\frac{5}{2}}\sqrt{289} = \sqrt{m^5289} = 17m^2\sqrt{m}$
- $9\sqrt{3m^2} + \sqrt{27} = 9m\sqrt{3} + 3\sqrt{3}$
- $3\sqrt{ab^2} - b\sqrt{a} = 3b\sqrt{a} - b\sqrt{a} = 2b\sqrt{a}$
- $\frac{4\sqrt{2n}}{\sqrt{16n^4}} = \frac{4\sqrt{2n}}{4n^2} = \frac{\sqrt{2n}}{n^2}$
- $\sqrt{\frac{225x^3}{49x}} = \frac{15x}{7}$
- $3\sqrt{44z} + \sqrt{99z} = 3\sqrt{4\cdot11z} + \sqrt{9\cdot11z} = 3 \cdot 2 \sqrt{11z} + 3 \sqrt{11z} = 9\sqrt{11z}$
- $\frac{\sqrt{8}}{1-\sqrt{3x}} = \frac{\sqrt{8}}{\sqrt{3x}} \cdot \frac{\sqrt{3x}}{\sqrt{3x}} = \frac{2\sqrt{2}\cdot\sqrt{3x}}{3x} = \frac{2\sqrt{6x}}{3x}$
    - $\frac{1}{\sqrt{a} - \sqrt{b}} \cdot \frac{\sqrt{a} + \sqrt{b}}{\sqrt{a} + \sqrt{b}}$
- $\sqrt{\frac{20}{121d^4}} = \sqrt{\frac{4\cdot5}{11^2d^4}} = \frac{2\sqrt{5}}{11 \cdot d^2}$
- $\sqrt{\frac{20}{121d^3}} = \frac{\sqrt{4 \cdot 5}}{11 \cdot d \sqrt{d}} = \frac{2\sqrt{5d}}{11d \cdot d}$
