# Chapter 1: Prerequisites
## 1.1 Real Numbers: Algebra Essentials
- `natural numbers`: numbers used for counting/enumerating items. Can use set notation $\{1, 2, 3, ...\}$
- `whole numbers`: the set of natural numbers plus zero: $\{0, 1, 2, 3, ...\}$
- `integers`: add to the set of whole numbers the opposites of each number $\{..., -3, -2, -1, 0, 1, 2, 3, ...\}$
  - Three subsets of integers, negative integers, zero, and positive integers
- `rational numbers`: fractions (or quotients) containing integers in both the numerator and the denominator, and the denominator can never be zero
  - $\{\frac{m}{n} | m\space\text{and}\space n\space\text{are integers and}\space n \ne 0\}$
- `terminating decimal`: $\frac{15}{8} = 1.875$
- `repeating decimal`: $\frac{4}{11} = 0.36363636... \space0.\overline{36}$
- `irrational numbers`: numbers that cannot be written as a fraction of two integers
  - $\{h | h \space\text{is not a rational number}\}$
- `real numbers`: the set of both rational and irrational numbers
  - Similar to integers, these can be divided into sets of negative real numbers, zero, and positive real numbers
  - You can put these numbers on a number line
- ![Sets of numbers](figure-01.2.jpg)
  - N: the set of natural numbers
  - W: the set of whole numbers
  - I: the set of integers
  - Q: the set of rational numbers
  - Q': the set of irrational numbers
### Performing Calculations Using the Order of Operations
- Order of operations must be evaluated in a systematic order, typical acronym is **PEMDAS**
  - **P**(arenthesis)
  - **E**(xponents)
  - **M**(ultiplication) and **D**(ivision)
  - **A**(ddition) and **S**(ubtraction)
- For a mathematical expression, simplify it using order of operations
  - Step 1. Simplify any expression with grouping symbols
  - Step 2. Simplify any expressions containing exponents or radicals
  - Step 3. Perform any multiplication in order, from left to right
  - Step 4. Perform any addition and subtraction in order, from left to right
### Using Properties of Real Numbers
- **Commutative properties are associated with repositioning**
  - For example, $5 + 2 = 2 + 5$ and $5 \cdot 2 = 2 \cdot 5$
  - `commutative property of addition`: numbers may be added in any order without affecting the sum
  - `commutative property of multiplication`: numbers may be multiplied in any order without affecting the product
- **Associative properties refer to regrouping**
  - $5 + (2 + 3) = (5 + 2) + 3$ and $5 \cdot (2 \cdot 3) = (5 \cdot 2) \cdot 3$
  - Or $a(bc) = (ab)c$
  - `associative property of multiplication`: does not matter how we group numbers when multiplying
  - `associative property of addition`: numbers may be grouped differently without affecting the sum
- Distributive property combines addition and multiplication
  - `distributive property`: the product of a factor times a sum is the sum of the factor times each term in the sum
  - $a \cdot (b + c) = a \cdot b + a \cdot c$
  - Ex: $15(121) = 15(100 + 20 + 1) = 15 \cdot 100 + 15 \cdot 20 + 15 \cdot 1 = 1500 + 300 + 15 = 1815$
  - Ex: $a(b + c - d + e) = ab + ac - ad + ae$
- Identity properties
  - `identity property of addition`: states that there is a unique number, called "additive identity" (0), that, when added to a number, results in the original number
    - $a + 0 = a$
  - `identity property of multiplication`: states that there is a unique number, called "multiplicative identity" (1), that, when multiplied by a number, results in the original number
    - $a \cdot 1 = a$
- Inverse properties
  - `inverse property of addition`: for every real number, there is a unique number that when added to the original number results in the additive identity(opposite)
    - $a + (-a) = 0$
  - `inverse property of multiplication`: for all real numbers (except 0), there is a unique number, called the "multiplicative inverse" (reciprocal) that, when multiplied by the original number, results in the multiplicative identity (1)
    - $a \cdot \frac{1}{a} = 1$
    - $\frac{3}{5} \cdot \frac{5}{3} = 1$
    - This does not apply to zero because $\frac{1}{0}$ is undefined
- Expression versus equation
  - An expression is something that does not have a "solution", you can simplify or evaluate
  - An equation is something that is "solved", if a sentence has "is" in it, it is an equation
- Examples
  - $12x^3y^7 - 9x^4y^2 - 2x^8y^3 = 3x^3y^2(4y^5 - 3x - x^5y)$
  - $2\pi r(r + h) = 2\pi r^2 + 2\pi rh$
  - $2(L + W) = 2L + 2W$
  - $4y^3 + y = y(4y^2 + 1)$
  - $2x^2y^3 - 4xy + 6x^7y^9 = 2xy(xy^2 - 2 + 3x^6y^8)$
  - $3x + 6 = 3(x + 2)$
  - $3x + 7 = 5(\frac{3}{5}x + \frac{7}{5})$
  - $17xy + 13x^3w = 7z(\frac{17xy}{7z} + \frac{13x^3w}{7z})$
  - $12 - 2(3 - (6 - 5)^2 + (4 - 5)^3 - 2 \div(3-5)) = 12 - 2(3 - 1 - 1 + 1) = 12 - 4 = 8$
  - $5l \div 3l \times (9-6) = \frac{5l}{3l} \times 3 = \frac{5}{3} \cdot \frac{3}{1} = 5$
  - $-5 + 2(3 - (4 - 5)^3 - (3 - 4)^2 + 3 \div(4-1) = -5 + 2(3 - -1 - 1 + 3 \div3) = -5 + 2(3 + 1 - 1 + 1) = -5 + 2(4) = -5 + 8 = 3$
    - If $a > 0 then a^{even or odd} = positive$
    - If $a < 0 and a^{even} = positive$ if $a < 0 and a^{odd} = negative$
### 1.1 Section Exercises
- $10 + 2 \times (5 - 3)$
- $6 \div 2 - (81 \div 3^2)$
## 1.2 Exponents and Scientific Notation
- Exponents is a base multiplied by itself multiple times
- $a^n = n^{th} power of a = n^{th} degree of a$
  - $a$ is the base and $n$ is our exponent/degree
  - Ex. $5^3 = 5 \cdot 5 \cdot 5$
- Multiplication of exponents (**with the same base!**) means you add
  - Ex. $2^3 \cdot 2^4 = 2 \cdot 2 \cdot 2 \cdot 2 \cdot 2 \cdot 2 \cdot 2$
- Division of exponents (**with the same base**) means you subtract
  - Ex. $\frac{2^5}{2^3} = \frac{2 \cdot 2 \cdot 2 \cdot 2 \cdot 2}{2 \cdot 2 \cdot 2} = 2^2$
  - Ex. $\frac{2^7}{2^11} = \frac{1}{2^4}$
    - In this instance, where do you have the higher degree of an exponent? If the denominator, you can subtract the powers from each other, then take the reciprocal
    - Negative exponent switches position
    - $\frac{a^{-1}}{1} = \frac{1}{a^n}$
- Ex. $\frac{2^{-3} \cdot 5^4 \cdot 7^{-2} \cdot 11^5}{3^{-5} \cdot 19^2} = \frac{5^4 \cdot 11^5 \cdot 3^5}{2^3 \cdot 7^2 \cdot 19^2}$
  - Note how $2^{-3}$, $7^{-2}$, and $3^{-5}$ were flipped to obtain positive exponents
- Ex. $\frac{2^5 \cdot 3^7 \cdot 5 \cdot 7^{11}}{2^4 \cdot 3^9 \cdot 5^12 \cdot 7^3} = \frac{2^1 \cdot 7^8}{3^2 \cdot 5^{11}}$
- $(a^n)^m = a^{n \cdot m}$
  - Ex. $(2^3)^4 = (2^3)(2^3)(2^3)(2^3) = 2^{12}$
- $(a^n \cdot b^m)^k = a^{n \cdot k}b^{m \cdot k}$
  - Ex. $(2^3 \cdot 3^4)^2 = (2^3 \cdot 3^4)(2^3 \cdot 3^4) = 2^6 \cdot 3^8$
  - Ex. $(5x^3y^5z)^2 = 5^{1 \cdot 2}\cdot x^{3 \cdot 2} \cdot y^{5 \cdot 2} \cdot z^{2}$
- $\frac{a}{b}^n = \frac{a^n}{b^n}$
- $\frac{a^n}{b^m}^k = \frac{a^{nk}}{b^{mk}}$
- Examples
  - $(-x^5y^2z)^3 = -x^{15}y^6z^3$
    - Don't forget the negative...
  - $(-x^{-2}y^2z^{-1})^{-2} = \frac{1}{(-x^{-2}y^2z^{-1})^2} = \frac{1}{x^{-4}y^4z^{-2}} = \frac{x^4z^2}{y^4}$
    - Don't forget the negatives
  - $(-x^{-2}y^2z^{-1})^{-2} = (-1)^{-2}x^4y^{-4}z^2 = \frac{x^4z^2}{y^4}$
  - $(3x^{-2}y^{-5}z)^{-3} = \frac{1}{(3x^{-2}y^{-5}z)^{3}} = \frac{1}{3^3x^{-6}y^{-15}z^3} = \frac{x^6y^{15}}{27z^3}$
  - $(3x^{-2}y^{-5}z)^{-3} = 3^{-3}x^6y^{15}z^{-3} = \frac{x^6y^{15}}{27z^3}$
  - $(-2x^{-2}y^2z^{-1})^{-2} = (-2)^{-2}x^4y^{-4}z^2 = \frac{x^4z^2}{-2^2y^4} = \frac{x^4z^2}{4y^4}$
- Any number to the first power is the number itself
  - $a^1 = a$
  - Ex: $(4x)^{-1} = \frac{1}{4x}$
  - Ex: $4x^{-1} = \frac{4}{x}$
  - Ex: $3 \cdot 2^{-4} = \frac{3}{2^4}$
- Any number (except zero) to the zero power is 1
  - $a^0 = 1$
- Any number (except 0) to the -1 power is 1 over the number
  - $a^{-1} = \frac{1}{a}$
- $(\frac{5x^3y^{-2}z^{-4}}{2x^7y^5z^{-9}})^{-2} = (\frac{5x^{-4}y^{-7}z^{5}}{2})^{-2} = (\frac{5^{-2}x^8y^{14}z^{-10}}{2^{-2}}) = \frac{4 \cdot x^8 \cdot y^{14}}{25 \cdot z^{10}}$
  - First step for this problem is to combine exponents with similar bases
- $(-2x^{-3}y^4z^1x^5y^{-3})^2(\frac{-x^4y^3}{x^7}) = (-2x^2yz)^2(-x^{-3}y^3) = (-2^2x^4y^2z^2)(-x^{-3}y^3) = -4xy^5z^2$
### Section 1.2 Examples
- $9^2 = 9 \cdot 9 = 81$
- $15^{-2} = \frac{1}{15^2} = \frac{1}{225}$
- $3^2 \times 3^3 = 3^5$
- $5^{-2} \div 5^2 = \frac{1}{5^2 \cdot 5^2} = \frac{1}{625}$
- $4^2 \times 4^3 \div 4^{-4} = \frac{4^5}{4^{-4}} = 4^{5 -(-4)}=4^9$
- $(12^3 \times 12)^{10} = (12^4)^{10}=12^{40}$
- $(y^7)^3 \div x^{14} = \frac{y^{21}}{x^{14}}$
- $\sqrt[5]{2^5} = 2^{\frac{5}{7}}$
- $(\sqrt{x})^2 = x^{\frac{1}{2}} x^{\frac{1}{2}} = x^1 = x$
- $\frac{a^3a^2}{a} = \frac{a^5}{a} = a^4$
- $\frac{(16\sqrt{x})^2}{y^{-1}} = \frac{(16^2x)}{y^{-1}} = 256xy$
- $\frac{2^3}{(3a)^{-2}} = 8 \cdot 9 \cdot a^2$
- $(\frac{3^2}{a^2})^{-2}(\frac{a^4}{2^2})^2n = (\frac{a^3}{9})^2(\frac{a^4}{4})^2 = (\frac{a^6}{81})(\frac{a^8}{16}) = \frac{a^{14}}{81 \cdot 16}$
- $(6^2 - 24)^2 \div (\frac{x}{y})^{-5} = 12^2 \div (\frac{y}{x})^5 = 12^2 \div \frac{y^5}{x^5} = 144 \cdot \frac{x^5}{y^5}$
- $\frac{m^2n^3}{a^2c^{-3}} \cdot \frac{a^{-7}n^{-2}}{m^2c^4} = \frac{m^{2 - 2} \cdot n^3 \cdot a^{-7-2}}{c^{-3+4}} = \frac{n^1 \cdot a^{-9}}{c} = \frac{n}{ca^9}$

## 1.3 Radicals and Rational Exponents
- In a square root, the symbol $\sqrt{}$ is the `radical`, the number under the radical is the `radicand`, and the entire expression is the `radical expression`
- If there is no number written, then there is an "invisible" two in the radical, ex. $\sqrt[2]{25}$
- In the example $\sqrt[n]{a^m}$
  - $n$ = index
  - $m$ = exponent
  - $a$ = base
  - $a^m$ = radicand
- $\sqrt{100} = 10$
- $\sqrt{\sqrt{16}} = \sqrt{4} = 2$
- $\sqrt{25 + 144} = \sqrt{169} = 13$
- $\sqrt{}$
- If a > 0 and b > 0, then $\sqrt{ab} = \sqrt{a} \cdot \sqrt{b}$
  - Similarly, $\sqrt[5]{a} \cdot \sqrt[5]{b} = \sqrt[5]{ab}$
- $\frac{\sqrt{234x^{11}y}}{\sqrt{26x7y}} = \sqrt{\frac{234x^{11}y}{26x^7y}} = \sqrt{\frac{117x^4}{13}} = \sqrt{9x^4} = 3x^2$
- $\sqrt{2} \cdot \sqrt{8} = \sqrt{2 \cdot 8} = \sqrt{16} = 4$
- $3\sqrt{17} + 2\sqrt{17} = 5\sqrt{17}$
  - Similar radicals can be combined (think of it as the same as $3x + 2x = 5x$)
- $\sqrt{5} + 6\sqrt{20}$
- $5\sqrt{2} + 3\sqrt{18} = 5\sqrt{2} + 3\sqrt{9 \cdot 2} = 5\sqrt{2} + 9\sqrt{2} = 14\sqrt{2}$
- $20\sqrt{72a^3b^4c} - 14\sqrt{8a^3b^4c} = 20\sqrt{36 \cdot 2 a^2 \cdot a^1 \cdot b^2 \cdot b^2 \cdot c} - 14\sqrt{4 \cdot 2 \cdot a^2 \cdot a \cdot b^2 \cdot b^2 \cdot c}$
  - $= 20 \cdot 6ab^2\sqrt{2ac} - 14 \cdot 2ab^2\sqrt{2ac} = 120ab^2\sqrt{2ac} - 28ab^2\sqrt{2ac} = 92ab^2\sqrt{2ac}$
- $\sqrt{a^4} = a^{\frac{4}{2}} = a^2$
- $\sqrt[3]{1000} = 10$
- This is an example of "not good technique" for simplifying square root expressions, very manual technique
  - $\sqrt{72a^7b^{11}c^5} = \sqrt{36 \cdot 2 \cdot a^2\cdot a^2\cdot a^2 \cdot a^1 \cdot b^2\cdot b^2\cdot b^2\cdot b^2\cdot b^2 \cdot b^1 \cdot c^2\cdot c^2 \cdot c^1} = 6aaabbbbbcc\sqrt{2abc} = 6a^3b^5c^2\sqrt{2abc}$
- This is an example of "good technique"
  1. Prime factorization of any numbers under the radicand
  2. Divide the exponents within the radical by the index of the radical
  3. Combine the results of refactoring
  - $\sqrt{72a^7b^{11}c^5} = \sqrt{2^3 \cdot 3^2a^7b^{11}c^5}$
    - Take the number under th radical and do prime factorization
      - ex. $72 = 2^3 \cdot 3^2$
    - Check the exponents of each prime factor
    - Divide the exponents within the radical by the index of the radical
      - $\sqrt{2^3} = 2\sqrt{2}$
      - $\sqrt{3^2} = 3$
      - $\sqrt{a^7} = a^3\sqrt{a}$
      - $\sqrt{b^{11}} = b^5\sqrt{b}$
      - $\sqrt{c^5} = c^2\sqrt{c}$
    - Combine the results of your refactoring
      - $6a^3b^5c^2\sqrt{2abc}$
    - Additional examples
      - $\sqrt[3]{a^5} = a\sqrt[3]{a^2}$
      - $\sqrt[5]{4a^4b^5c^6e^7d^8w^{13}p^{26}}$
        - Prime factorization
          - $\sqrt[5]{4} = 2 \cdot 2 = \sqrt[5]{2^2}$
        - Divide exponents by the index
          - $\sqrt[5]{a^4}$
          - $\sqrt[5]{b^5} = b$
          - $\sqrt[5]{c^6} = c\sqrt[5]{c}$
          - $\sqrt[5]{e^7} = e\sqrt[5]{e^2}$
          - $\sqrt[5]{d^8} = d\sqrt[5]{d^3}$
          - $\sqrt[5]{w^{13}} = w^2\sqrt[5]{w^3}$
          - $\sqrt[5]{p^{26}} = p^5\sqrt[5]{p}$
        - Combine
          - $bcedw^2p^5\sqrt[5]{2^2ce^2d^3w^3p}$
      - $\sqrt[3]{432a^7b^2c^{11}de^{15}} = \sqrt[3]{2^4 \cdot 3^3 \cdot a^7b^2c^{11}de^{15}}$
        - Prime factorization
          - $432 / 2 = 216$
            - $216 / 2 = 108$
              - $108 / 2 = 54$
                - $54 / 2 = 27$
                  - $27 / 3 = 9$
                    - $9 / 3 = 3$
          - result = $2^4 \cdot 3^3$
        - Divide exponents by the index
          - $\sqrt[3]{2^4} = 2\sqrt[3]{2}$
          - $\sqrt[3]{3^3} = 3$
          - $\sqrt[3]{a^7} = a^2\sqrt[3]{a}$
          - $\sqrt[3]{b^2} = \sqrt[3]{b^2}$
          - $\sqrt[3]{c^{11}} = c^3\sqrt[3]{c^2}$
          - $\sqrt[3]{d} = \sqrt[3]{d}$
          - $\sqrt[3]{e^{15}} = e^5$
        - Combine
          - $6a^2c^3e^5\sqrt[3]{2ab^2c^2d}$
- Can think of the square root as the opposite of squaring a number
  - $\sqrt{4} = 2$
  - You can however, have $-\sqrt{25} = -5$
- **PRINCIPAL SQUARE ROOT**
  - The principal square root of $a$ is the non-negative number that, when multiplied by itself, equals $a$
  - When we say $\sqrt{4}$, it is a number, and an expression, and it is only positive
    - This is different from when we say $x^2 = 4$, this is an equation and may have multiple answers
      - Ex. $x^2 = 4 = \pm2$
- **Under any square root (or any even root), the radicand must be positive**
  - You cannot say $\sqrt{-25}$, this is called "not real"
- **IMPORTANT RULE**
  - When dealing with even roots, you need to make sure that the radicand is positive, this is because the radicand could be positive or negative, so we agree that it is positive
  - $\sqrt{a^2} = |a|$
    - Absolute value indicates "distance" from zero
  - $\sqrt{(-2)^2} = |-2| = 2$
  - $\sqrt[2]{(-6)^2} = |-6| = 6$
  - $\sqrt[2]{a^{14}} = |a^7|$
  - When dealing with odd roots, you do not have the possibility of having two options
  - $\sqrt[3]{a^3}$
- Under even root, in order to continue, you must have positive radicands
### Examples
- For examples in the textbook, assume all variables are positive
- $(\frac{\sqrt{250x^2}}{\sqrt{100b^3}})(\frac{7\sqrt{b}}{\sqrt{125x}}) = \sqrt{\frac{250x^2}{100b^3}} \cdot \frac{7}{1} \cdot \sqrt{\frac{b}{125x}} = \sqrt{\frac{5x^2}{2b^3}} \cdot \frac{7}{1} \cdot \sqrt{\frac{b}{125x}} = 7 \cdot \sqrt{\frac{5 \cdot x^2}{2 \cdot b^3} \cdot \frac{6}{125x}} = 7 \cdot \sqrt{\frac{x}{2 \cdot b^2 \cdot 25}} = 7 \cdot \frac{\sqrt{x}}{5b\sqrt{2}} = \frac{7\sqrt{x}}{5b\sqrt{2}} = \frac{7\sqrt{2x}}{10b}$
  - Remember to rationalize denominator before you are done
## 1.4 Polynomials

## 1.5 Factoring Polynomials
## 1.6 Rational Expressions