## 1.2 Exponents and Scientific Notation
### Using the Product Rule of Exponents
- When multiplying exponential expressions with the same base, we write the result with the common base and add the exponents
- **Product rule of exponents**: for any real number $a$ and natural numbers $m$ and $n$, the product rule of exponents states that $a^m \cdot a^n = a^{m+n}$
- Example: $x^3 \cdot x^4 = x^{3 + 4} = x^7$
- Example: $2^3 \cdot 2^4 = 2^7$
### Using the Quotient Rule of Exponents
- Allows us to simplify an expression that divides two numbers with the same base, but different exponents. When dividing exponential expressions with the same base, we write the result with the common base and subtract the exponents
- **Quotient rule of exponents**: for any real number $a$ and natural numbers $m$ and $n$, such that $m > n$, the quotient rule of exponents states that $\frac{a^m}{a^n} = a^{m-n}$
- Example: $\frac{y^9}{y^5} = y^{9-5} = y^4$
- Example: $\frac{(-2)^14}{(-2)^9} = (-2)^5
### Using the Power Rule of Exponents
- If an exponential expression is raised to a power, we multiply the expression inside the parentheses by the outer exponent. Be careful to distinguish this rule from the product rule, for example $5^3 \cdot 5^4 = 5^7$ but $(5^3)^4 = 5^{12}$
- **Power rule of exponents**: for any real number $a$ and positive integers $m$ and $n$, the power rule of exponents states that $(a^m)^n = a^{m \cdot n}$
- Example: $(x^2)^3 = x^2 \cdot x^2 \cdot x^2 = x^6$
### Using the Zero Exponent Rule of Exponents
- If the exponents $m$ and $n$ in the quotient rule are equal to each other, we simplify the expression to 1
- **Zero exponent rule of exponents**: For any nonzero real number $a$, the zero exponent rule of exponents states that $a^0 = 1$
- Example: $\frac{t^8}{t^8} = t^{8-8} = t^0$ any nonzero real number raised to the zeroth power is equal to 1
### Using the Negative Rule of Exponents
- If we divide a smaller exponential expression by a larger one, we end up with a negative exponent, we can simplify this expression by taking its reciprocal
- **Negative rule of exponents**: For any nonzero real number $a$ and natural number $n$, the negative rule of exponents states that $a^{-n} = \frac{1}{a^n}$
- Example: $\frac{h^3}{h^5} = \frac{h \cdot h \cdot h}{h \cdot h \cdot h \cdot h \cdot h} = \frac{1}{h^2}$
- Example: $\frac{h^3}{h^5} = h^{3-5} = h^{-2} = \frac{1}{h^2}$
### Finding the Power of a Product


---
In-class Notes

### Section 1.2 Examples
- $9^2 = 9 \cdot 9 = 81$
- $15^{-2} = \frac{1}{15^2} = \frac{1}{225}$
- $3^2 \times 3^3 = 3^5$
- $5^{-2} \div 5^2 = \frac{1}{5^2 \cdot 5^2} = \frac{1}{625}$
- $4^2 \times 4^3 \div 4^{-4} = \frac{4^5}{4^{-4}} = 4^{5 -(-4)}=4^9$
- $(12^3 \times 12)^{10} = (12^4)^{10}=12^{40}$
- $(y^7)^3 \div x^{14} = \frac{y^{21}}{x^{14}}$
- $\sqrt[5]{2^5} = 2^{\frac{5}{7}}$
- $(\sqrt{x})^2 = x^{\frac{1}{2}} x^{\frac{1}{2}} = x^1 = x$
- $\frac{a^3a^2}{a} = \frac{a^5}{a} = a^4$
- $\frac{(16\sqrt{x})^2}{y^{-1}} = \frac{(16^2x)}{y^{-1}} = 256xy$
- $\frac{2^3}{(3a)^{-2}} = 8 \cdot 9 \cdot a^2$
- $(\frac{3^2}{a^2})^{-2}(\frac{a^4}{2^2})^2n = (\frac{a^3}{9})^2(\frac{a^4}{4})^2 = (\frac{a^6}{81})(\frac{a^8}{16}) = \frac{a^{14}}{81 \cdot 16}$
- $(6^2 - 24)^2 \div (\frac{x}{y})^{-5} = 12^2 \div (\frac{y}{x})^5 = 12^2 \div \frac{y^5}{x^5} = 144 \cdot \frac{x^5}{y^5}$
- $\frac{m^2n^3}{a^2c^{-3}} \cdot \frac{a^{-7}n^{-2}}{m^2c^4} = \frac{m^{2 - 2} \cdot n^3 \cdot a^{-7-2}}{c^{-3+4}} = \frac{n^1 \cdot a^{-9}}{c} = \frac{n}{ca^9}$
